Veir/Dialects/LLZK/String/OpInfo.lean
@@ -1,0 +1,72 @@
+module
+
+public import Veir.IR.Simp
+public import Veir.IR.OpInfo
+public import Veir.Verifier.Basic
+public import Veir.Dialects.LLZK.String.Properties
+meta import Veir.Meta.OpCode
+
+namespace Veir
+
+public section
+
+namespace LLZK
+
+@[opcodes]
+inductive String where
+| new
+deriving Inhabited, Repr, Hashable, DecidableEq
+
+end LLZK
+
+@[expose, properties_of]
+def LLZK.String.propertiesOf (op : LLZK.String) : Type :=
+match op with
+| .new => StringNewProperties
+
+def LLZK.String.fromAttrDict
+    (op : LLZK.String) (attrDict : Std.HashMap ByteArray Attribute) :=
+  match op with
+  | .new => StringNewProperties.fromAttrDict attrDict
+
+def LLZK.String.toAttrDict
+    (op : LLZK.String) (props : LLZK.String.propertiesOf op) :
+    Std.HashMap ByteArray Attribute :=
+  match op with
+  | .new =>
+    (Std.HashMap.emptyWithCapacity 1).insert
+      "value".toUTF8 (Attribute.stringAttr props.value)
+
+@[get_effects]
+def LLZK.String.getEffects
+    (_op : LLZK.String) (_props : LLZK.String.propertiesOf _op) : MemoryEffects :=
+  .none
+
+def LLZK.String.isConstantLike (_op : LLZK.String) : Bool := true
+
+def LLZK.String.hasSSADominance (_op : LLZK.String) (_index : Nat) : Bool := true
+
+#generate_dialect LLZK.String
+
+instance : IsOpCode LLZK.String where
+  fromName := LLZK.String.fromName
+  name := LLZK.String.name
+  propertiesOf := LLZK.String.propertiesOf
+  fromAttrDict := LLZK.String.fromAttrDict
+  toAttrDict := LLZK.String.toAttrDict
+
+def LLZK.String.verifyLocalInvariants {OpInfo : Type} [IsOpCode OpInfo]
+    [HasDialect OpInfo LLZK.String] (opType : LLZK.String) (op : OperationPtr)
+    (ctx : WfIRContext OpInfo) (opIn : op.InBounds ctx.raw) := do
+  match opType with
+  | .new => op.verifyPlainOpCounts ctx opIn 0 1
+
+instance : HasOpInfo LLZK.String where
+  verifyLocalInvariants := LLZK.String.verifyLocalInvariants
+  getEffects := LLZK.String.getEffects
+  isConstantLike := LLZK.String.isConstantLike
+  hasSSADominance := LLZK.String.hasSSADominance
+
+end
+
+end Veir
